WIP

src/RawRenaming.v
@@ -1,59 +1,164 @@
 Require Import Label PeanoNat Psatz Ring Compare_dec StrictProp.
 Require Import Var.
 
-Inductive raw_renaming :=
-  | raw_renaming_id : raw_renaming
-  | raw_renaming_extend :
-      var -> raw_renaming -> var -> raw_renaming.
+Definition incoming_item : Set := (option label) * nat.
 
-Fixpoint apply_raw_renaming_var r : var_op 0 0 :=
-  match r with
-  | raw_renaming_id => var_op_id
-  | raw_renaming_extend vl r vr =>
-    pop_var vl @ lift_var_op (apply_raw_renaming_var r) @ push_var vr
+Definition incoming := list incoming_item.
+
+Definition apply_incoming_item
+           (vn : var + nat) (inc : incoming_item)
+  : var + nat :=
+  match vn with
+  | inl v =>
+    match inc with
+    | (l, m) =>
+      if label_opt_eqb l (v_label_opt v) then
+        match v_nat v with
+        | 0 => inr m
+        | S n => inl (mk_var (v_label_opt v) n)
+        end
+      else
+        vn
+    end
+  | inr n => vn
   end.
 
-Set Primitive Projections.
-Record renaming_rhs :=
-  mk_renaming_rhs {
-      rhs_raw_renaming : raw_renaming;
-      rhs_push : var
-    }.
-Add Printing Constructor renaming_rhs.
-Unset Primitive Projections.
+Definition apply_incoming inc vn :=
+  List.fold_left apply_incoming_item inc vn.
 
-Definition renaming_rhs_extend vl r vr :=
-  mk_renaming_rhs
-    (raw_renaming_extend vl
-        (rhs_raw_renaming r)
-        (unshift_var (rhs_push r) vr))
-    (shift_var vr (rhs_push r)).
+Lemma apply_incoming_cons_inv hd tl vn :
+  apply_incoming (cons hd tl) vn
+  = apply_incoming tl (apply_incoming_item vn hd).
+Proof. reflexivity. Qed.
 
-Fixpoint transpose_push_raw_renaming v r {struct r} :=
-  match r with
-  | raw_renaming_id => mk_renaming_rhs raw_renaming_id v
-  | raw_renaming_extend vl r vr =>
-    if var_eqb v vl then mk_renaming_rhs r vr
-    else renaming_rhs_extend
-           (unshift_var v vl)
-           (transpose_push_raw_renaming (unshift_var vl v) r)
-           vr
+Definition incoming_item_less_than
+           (n : nat) (inc : incoming_item) :=
+  Nat.ltb (snd inc) n.
+
+Definition incoming_less_than (n : nat) (inc : incoming) :=
+  List.forallb (incoming_item_less_than n) inc.
+
+Lemma incoming_less_than_cons_inv n hd tl :
+  incoming_less_than n (cons hd tl)
+  = andb (incoming_item_less_than n hd)
+         (incoming_less_than n tl).
+Proof. reflexivity. Qed.
+
+Definition incoming_item_is_less_than n inc : SProp :=
+  if incoming_item_less_than n inc then sUnit
+  else sEmpty.
+
+Definition incoming_is_less_than n inc : SProp :=
+  if incoming_less_than n inc then sUnit
+  else sEmpty.
+
+Lemma incoming_is_less_than_head n inc rest :
+  incoming_is_less_than n (inc :: rest)%list ->
+  incoming_item_is_less_than n inc.
+Proof.
+  unfold incoming_is_less_than, incoming_item_is_less_than.
+  rewrite incoming_less_than_cons_inv.
+  destruct incoming_item_less_than; easy.
+Qed.
+
+Lemma incoming_is_less_than_tail n inc rest :
+  incoming_is_less_than n (inc :: rest)%list ->
+  incoming_is_less_than n rest.
+Proof.
+  unfold incoming_is_less_than, incoming_item_is_less_than.
+  rewrite incoming_less_than_cons_inv.
+  destruct incoming_item_less_than; easy.
+Qed.
+
+Definition outgoing_item := option label.
+
+Definition outgoing := list outgoing_item.
+
+Definition apply_outgoing_item
+           (vn : var + nat) (otg : option label)
+  : var + nat :=
+  match vn with
+  | inr n =>
+    match n with
+    | 0 => inl (mk_var otg 0)
+    | S n => inr n
+    end
+  | inl v =>
+    if label_opt_eqb otg (v_label_opt v) then
+      inl (mk_var (v_label_opt v) (S (v_nat v)))
+    else
+      vn
   end.
 
-Fixpoint compose_raw_renaming r1 r2 :=
-  match r1 with
-  | raw_renaming_id => r2
-  | raw_renaming_extend vl r1 vr =>
-    let rhs := transpose_push_raw_renaming vr r2 in
-    raw_renaming_extend
-      vl
-      (compose_raw_renaming r1 (rhs_raw_renaming rhs))
-      (rhs_push rhs)
+Definition apply_outgoing otg vn :=
+  List.fold_left apply_outgoing_item otg vn.
+
+Lemma apply_outgoing_cons_inv hd tl vn :
+  apply_outgoing (cons hd tl) vn
+  = apply_outgoing tl (apply_outgoing_item vn hd).
+Proof. reflexivity. Qed.
+
+Definition vn_less_than n (vn : var + nat) :=
+  match vn with
+  | inl _ => true
+  | inr m => Nat.ltb m n
   end.
 
-Fixpoint inverse_raw_renaming r :=
-  match r with
-  | raw_renaming_id => r
-  | raw_renaming_extend vl r vr =>
-      raw_renaming_extend vr (inverse_raw_renaming r) vl
-  end.
+Definition vn_is_less_than n vn : SProp :=
+  if vn_less_than n vn then sUnit
+  else sEmpty.
+
+Lemma vn_is_less_than_inr_succ n m :
+  vn_is_less_than (S n) (inr (S m)) ->
+  vn_is_less_than n (inr m).
+Proof. induction n; easy. Qed.
+
+Lemma apply_incoming_less_than n inc vn :
+  incoming_is_less_than n inc ->
+  vn_is_less_than n vn ->
+  vn_is_less_than n (apply_incoming inc vn).
+Proof.
+  intro Hinc.
+  generalize dependent vn.
+  induction inc as [|[l m] tl]; intros vn Hv; try easy.
+  apply incoming_is_less_than_head in Hinc as Hinc1.
+  apply incoming_is_less_than_tail in Hinc as Hinc2.
+  rewrite apply_incoming_cons_inv.
+  apply (IHtl Hinc2).
+  destruct vn as [v|o]; cbn; try easy.
+  destruct label_opt_eqb, (v_nat v); easy.
+Qed.
+
+Lemma apply_outgoing_less_than n otg vn :
+  vn_is_less_than (n + List.length otg) vn ->
+  vn_is_less_than n (apply_outgoing otg vn).
+Proof.
+  generalize dependent vn.
+  induction otg as [|l tl]; intros vn Hv.
+  - rewrite <- plus_n_O in Hv; easy.
+  - rewrite apply_outgoing_cons_inv.
+    apply IHtl.
+    destruct vn as [v|[|m]]; cbn; try easy.
+    + destruct label_opt_eqb; easy.
+    + cbn in Hv.
+      rewrite <- plus_n_Sm in Hv.
+      apply vn_is_less_than_inr_succ; easy.
+Qed.
+
+Lemma apply_renaming_var_less_than v inc otg :
+  incoming_is_less_than (List.length otg) inc ->
+  vn_is_less_than 0
+    (apply_outgoing otg (apply_incoming inc (inl v))).
+Proof.
+  intros Hin.
+  apply apply_outgoing_less_than.
+  apply apply_incoming_less_than; easy.
+Qed.
+
+Definition apply_renaming inc otg
+           {H : incoming_is_less_than (List.length otg) inc}
+           v :=
+  match apply_outgoing otg (apply_incoming inc (inl v)) with
+  | inl v' => v'
+  | inr _ => 
+
